add can full invertibility

hseq.v
@@ -8,7 +8,8 @@ Require Import Rpos.
 Require Import term.
 
 Require Import List.
-Require Import Permutation.
+Require Import Permutation_more.
+Require Import Permutation_solve.
 Require Import Lra.
 
 Local Open Scope Rpos_scope.
@@ -38,6 +39,12 @@ Fixpoint sum_vec (l : list Rpos) :=
   | r :: l => Rplus (projT1 r) (sum_vec l)
   end.
 
+Fixpoint mul_vec (l : list Rpos) r :=
+  match l with
+  | nil => nil
+  | r0 :: l => (time_pos r r0) :: (mul_vec l r)
+  end.
+
 Lemma sum_vec_le_0 : forall r, (0 <= sum_vec r)%R.
   induction r; [ | move : a=> [a Ha]; simpl;  apply (R_blt_lt 0 a) in Ha]; simpl; try nra.
 Qed.
@@ -51,30 +58,117 @@ Lemma sum_vec_non_nil : forall r, r <> nil -> (0 <? sum_vec r)%R = true.
   pose Hle := (sum_vec_le_0 r).
   nra.
 Qed.
-
 (** ** Hypersequent *)
 
 Definition hypersequent : Set := list sequent.
 
-Inductive HR : hypersequent -> Type :=
-| INIT : HR (nil :: nil)
-| W : forall G T, HR G -> HR (T :: G)
-| C : forall G T, HR (T :: T :: G) -> HR (T :: G)
-| S : forall G T1 T2, HR ((T1 ++ T2) :: G) -> HR (T1 :: T2 :: G)
-| M : forall G T1 T2, HR (T1 :: G) -> HR (T2 :: G) -> HR ((T1 ++ T2) :: G)
-| T : forall G T r, HR (seq_mul r T :: G) -> HR (T :: G)
-| ID : forall G T n r s, HR (T :: G) -> sum_vec r = sum_vec s -> HR ((vec s (covar n) ++ vec r (var n) ++ T) :: G)
-| plus : forall G T A B r, HR ((vec r A ++ vec r B ++ T) :: G) -> HR ((vec r (A +S B) ++ T) :: G)
-| max : forall G T A B r, HR ((vec r B ++ T) :: (vec r A ++ T) :: G) -> HR ((vec r (A \/S B) ++ T) :: G)
-| min : forall G T A  B r, HR ((vec r A ++ T) :: G) -> HR ((vec r B ++ T) :: G) -> HR ((vec r (A /\S B) ++ T) :: G)
-| ex_seq : forall G T1 T2, Permutation T1 T2 -> HR (T1 :: G) -> HR (T2 :: G)
-| ex_hseq : forall G H, Permutation G H -> HR G -> HR H.
+Inductive HR b : hypersequent -> Type :=
+| INIT : HR b (nil :: nil)
+| W : forall G T, HR b G -> HR b (T :: G)
+| C : forall G T, HR b (T :: T :: G) -> HR b (T :: G)
+| S : forall G T1 T2, HR b ((T1 ++ T2) :: G) -> HR b (T1 :: T2 :: G)
+| M : forall G T1 T2, HR b (T1 :: G) -> HR b (T2 :: G) -> HR b ((T1 ++ T2) :: G)
+| T : forall G T r, HR b (seq_mul r T :: G) -> HR b (T :: G)
+| ID : forall G T n r s, sum_vec r = sum_vec s -> HR b (T :: G) -> HR b ((vec s (covar n) ++ vec r (var n) ++ T) :: G)
+| Z : forall G T r, HR b (T :: G) -> HR b ((vec r zero ++ T) :: G)
+
+| plus : forall G T A B r, HR b ((vec r A ++ vec r B ++ T) :: G) -> HR b ((vec r (A +S B) ++ T) :: G)
+| mul : forall G T A r0 r, HR b ((vec (mul_vec r r0) A ++ T) :: G) -> HR b ((vec r (r0 *S A) ++ T) :: G)
+| max : forall G T A B r, HR b ((vec r B ++ T) :: (vec r A ++ T) :: G) -> HR b ((vec r (A \/S B) ++ T) :: G)
+| min : forall G T A  B r, HR b ((vec r A ++ T) :: G) -> HR b ((vec r B ++ T) :: G) -> HR b ((vec r (A /\S B) ++ T) :: G)
+| ex_seq : forall G T1 T2, Permutation T1 T2 -> HR b (T1 :: G) -> HR b (T2 :: G)
+| ex_hseq : forall G H, Permutation G H -> HR b G -> HR b H
+| can {f : b = true} : forall G T A r s, sum_vec r = sum_vec s -> HR b ((vec s (-S A) ++ vec r A ++ T) :: G) -> HR b (T :: G).
 
 (* Some basic properties *)
 
-Lemma HR_not_empty : forall G, HR G -> G <> nil.
+Lemma HR_not_empty b : forall G, HR b G -> G <> nil.
 Proof.
   move => G pi; induction pi; (try by []).
   move => Heq; apply IHpi; apply Permutation_nil.
   symmetry; by rewrite <- Heq.
 Qed.
+
+
+Lemma HR_no_can_can : forall G, HR false G -> HR true G.
+Proof.
+  move => G pi.
+  induction pi; try now constructor.
+  - apply T with r; apply IHpi.
+  - apply ex_seq with T1; assumption.
+  - apply ex_hseq with G; assumption.
+Qed.
+
+Lemma W_gen b : forall G H, HR b G -> HR b (H ++ G).
+Proof.
+  move => G H; move: G; induction H => G pi.
+  - auto.
+  - simpl; apply W; apply IHlist; apply pi.
+Qed.
+
+Lemma ID_gen b : forall G T A r s, sum_vec r = sum_vec s -> HR b (T :: G) -> HR b ((vec s (-S A) ++ vec r A ++ T) :: G).
+Proof.
+  move => G T A; move: G T.
+  induction A => G T r0 s Heq pi; unfold minus; fold minus.
+  - apply ID; assumption.
+  - apply ex_seq with (vec r0 (covar n) ++ vec s (var n) ++ T); [ perm_solve | ].
+    apply ID; try symmetry; assumption.
+  - apply Z; apply Z; apply pi.
+  - apply plus.
+    apply ex_seq with (vec r0 (A1 +S A2) ++ vec s (-S A1) ++ vec s (-S A2) ++ T); [ perm_solve | ].
+    apply plus.
+    eapply ex_seq.
+    2:{ eapply IHA1; [ apply Heq | ].
+        eapply ex_seq.
+        2:{ eapply IHA2; [ apply Heq | apply pi ]. }
+        perm_solve. }
+    perm_solve.
+  - apply mul.
+    eapply ex_seq with (vec r0 (r *S A) ++ vec (mul_vec s r) (-S A) ++ T) ; [ perm_solve | ].
+    apply mul.
+    apply ex_seq with (vec (mul_vec s r) (-S A) ++ vec (mul_vec r0 r) A ++ T); [ perm_solve | ].
+    apply IHA ; [ | apply pi].
+    (* TODO MOVING *)
+    have sum_mul_vec : forall l r, sum_vec (mul_vec l r) =  Rmult (projT1 r) (sum_vec l).
+    { clear.
+      induction l; move => [r Hr].
+      - simpl; nra.
+      - set t := (existT (fun r0 : R => (0 <? r0)%R = true) r Hr).
+        unfold mul_vec; fold (mul_vec l t).
+        unfold sum_vec; fold (sum_vec (mul_vec l t)); fold (sum_vec l).
+        rewrite IHl.
+        unfold t.
+        destruct a.
+        simpl.
+        nra. }
+    rewrite ? sum_mul_vec.
+    destruct r as [r Hr].
+    simpl.
+    apply R_blt_lt in Hr.
+    nra.
+  - apply min.
+    + apply ex_seq with (vec r0 (A1 \/S A2) ++ vec s (-S A1) ++ T); [perm_solve | ].
+      apply max.
+      apply W.
+      eapply ex_seq; [ | apply IHA1; [ apply Heq | apply pi] ].
+      perm_solve.
+    + apply ex_seq with (vec r0 (A1 \/S A2) ++ vec s (-S A2) ++ T); [perm_solve | ].
+      apply max.
+      apply ex_hseq with ((vec r0 A1 ++ vec s (-S A2) ++ T) :: (vec r0 A2 ++ vec s (-S A2) ++ T) :: G) ; [ perm_solve | ]. 
+      apply W.
+      eapply ex_seq; [ | apply IHA2; [ apply Heq | apply pi] ].
+      perm_solve.
+  - apply ex_seq with (vec r0 (A1 /\S A2) ++ vec s (-S A1 \/S -S A2) ++ T); [ perm_solve | ].
+    apply min.
+    + apply ex_seq with (vec s (-S A1 \/S -S A2) ++ vec r0 (A1) ++ T); [perm_solve | ].
+      apply max.
+      apply W.
+      apply IHA1; [ apply Heq | apply pi].
+    + apply ex_seq with (vec s (-S A1 \/S -S A2) ++ vec r0 (A2) ++ T); [perm_solve | ].
+      apply max.
+      apply ex_hseq with ((vec s (-S A1) ++ vec r0 A2 ++ T) :: (vec s (-S A2) ++ vec r0 A2 ++ T) :: G) ; [ perm_solve | ]. 
+      apply W.
+      eapply ex_seq; [ | apply IHA2; [ apply Heq | apply pi] ].
+      perm_solve.
+Qed.
+      
